WIP Start on Capture Sets Part 2

CaptureSets.v
@@ -9,277 +9,740 @@ Require Import OrderedType.
 Require Import FSetFacts.
 Require Import Atom.
 Require Import Nat.
+Require Import Bool.
 
-Declare Scope cset_scope.
+Create HintDb csets.
 
-(** A captureset -- a pair of free variables and bound variables. *)
-Inductive captureset : Type :=
-  | cset_universal : captureset
-  | cset_set : atoms -> nats -> captureset.
 
-Definition empty_cset := cset_set {} {}N.
-Definition universal_cset := cset_universal.
+(** ************************************************** *)
+(** Definition of Capture Sets *)
+(** ************************************************** *)
+
+(** A captureset -- a pair of triple of free variables,
+    bound variables, and if we contain the special
+    `universal` variable. *)
+Inductive cap : Type :=
+  | cset_set : atoms -> nats -> bool -> cap.
+
+
+(** ************************************************** *)
+(** Constructors *)
+(** ************************************************** *)
+
+Definition empty_cset := cset_set {} {}N false.
 
 (** The empty set may be written similarly to informal practice. *)
 Notation "{}C" :=
   empty_cset : metatheory_scope.
-Notation "{*}C" :=
-  universal_cset : metatheory_scope.
-
-(** Accessors *)
-Definition cset_fvars (c : captureset) : atoms :=
-  match c with
-  | cset_universal => {}
-  | cset_set A N => A
-  end.
-
-Definition cset_bvars (c : captureset) : nats :=
-  match c with
-  | cset_universal => {}N
-  | cset_set A N => N
-  end.
-
-(** Lifts predicates on sets of captures to non-universal capture sets **)
-Definition cset_vars (pf : atoms -> Prop)  (pb : nats -> Prop) (c : captureset) : Prop :=
-  match c with
-  | cset_set A N => pf A /\ pb N
-  | cset_universal => False
-  end.
-
-(* Could be implemented in terms of cset_vars but that leaves us with a dangeling /\ True *)
-Definition cset_all_fvars (p : atoms -> Prop) (c : captureset) : Prop :=
-  match c with
-  | cset_set A N => p A
-  | cset_universal => False
-  end.
-
-
-Definition cset_all_bvars (p : nats -> Prop) (c : captureset) : Prop :=
-  match c with
-  | cset_set A N => p N
-  | cset_universal => False
-  end.
 
 (** Singletons *)
 Definition cset_fvar (a : atom) :=
-  (cset_set (AtomSet.F.singleton a) (NatSet.F.empty)).
+  (cset_set (AtomSet.F.singleton a) NatSet.F.empty false).
+  
 Definition cset_bvar (k : nat) :=
-  (cset_set (AtomSet.F.empty) (NatSet.F.singleton k)).
+  (cset_set AtomSet.F.empty (NatSet.F.singleton k) false).
+
+Definition cset_universal :=
+  (cset_set AtomSet.F.empty NatSet.F.empty true).
+
+(** ************************************************** *)
+(** Selectors *)
+(** ************************************************** *)
+
+Definition cset_fvars (c : cap) : atoms :=
+  match c with
+  | cset_set A _ _ => A
+  end.
+
+Definition cset_bvars (c : cap) : nats :=
+  match c with
+  | cset_set _ N _ => N
+  end.
+
+Definition cset_has_universal (c : cap) : bool :=
+  match c with
+  | cset_set _ _ R => R
+  end.
+
+
+
+(** ************************************************** *)
+(** Operations *)
+(** ************************************************** *)
+
+(* Definition cset_lvar (l : atom) :=
+  (cset_set AtomSet.F.empty NatSet.F.empty (AtomSet.F.singleton l)). *)
 
 (** Predicates for determining if a capture set explicity references
     a variable -- used for determining if a capture set is well formed.
     Don't use these predicates for determining if a capture set
     captures a variable, as one needs to also test cset_universal. *)
-Definition cset_references_bvar (k : nat) (c : captureset) :=
-  cset_all_bvars (NatSet.F.In k) c.
+Definition cset_references_bvar (k : nat) (c : cap) :=
+  NatSet.F.In k (cset_bvars c).
 
-Definition cset_references_fvar (a : atom) (c : captureset) :=
-  cset_all_fvars (AtomSet.F.In a) c.
+Definition cset_references_fvar (a : atom) (c : cap) :=
+  AtomSet.F.In a (cset_fvars c).
 
-Definition cset_references_bvar_dec (k : nat) (c : captureset) :=
-  match c with
-  | cset_universal => false
-  | cset_set A N => NatSet.F.mem k N
-  end.
+Definition cset_references_bvar_dec (k : nat) (c : cap) :=
+  NatSet.F.mem k (cset_bvars c).
 
-Definition cset_references_fvar_dec (a : atom) (c : captureset) :=
-  match c with
-  | cset_universal => false
-  | cset_set A N => AtomSet.F.mem a A
-  end.
+Definition cset_references_fvar_dec (a : atom) (c : cap) :=
+  AtomSet.F.mem a (cset_fvars c).
 
-Lemma cset_references_bvar_eq (k : nat) (c : captureset) :
-  cset_references_bvar_dec k c = true <-> cset_references_bvar k c.
-Proof.
-  destruct c ; simpl ; intuition.
-Qed.
+Definition cset_remove_bvar (k : nat) (c : cap) : cap :=
+  cset_set (cset_fvars c) (NatSet.F.remove k (cset_bvars c)) (cset_has_universal c).
 
-Lemma cset_references_fvar_eq (k : atom) (c : captureset) :
-  cset_references_fvar_dec k c = true <-> cset_references_fvar k c.
-Proof.
-  destruct c ; simpl ; intuition.
-Qed.
+Definition cset_remove_fvar (a : atom) (c : cap) : cap :=
+  cset_set (AtomSet.F.remove a (cset_fvars c)) (cset_bvars c) (cset_has_universal c).
 
-Lemma cset_not_references_bvar_eq (k : nat) (c : captureset) :
-  cset_references_bvar_dec k c = false <-> ~ cset_references_bvar k c.
-Proof.
-  destruct c ; simpl.
-  - intuition.
-  - rewrite <- NatSetFacts.not_mem_iff. intuition.
-Qed.
-
-Lemma cset_not_references_fvar_eq (k : atom) (c : captureset) :
-  cset_references_fvar_dec k c = false <-> ~ cset_references_fvar k c.
-Proof.
-  destruct c ; simpl.
-  - intuition.
-  - rewrite <- AtomSetFacts.not_mem_iff. intuition.
-Qed.
-
-
-(** More predicates *)
-Definition empty_cset_bvars (c : captureset) : Prop :=
-  cset_all_bvars NatSet.F.Empty c.
-Definition empty_cset_fvars (c : captureset) : Prop :=
-  cset_all_fvars AtomSet.F.Empty c.
-
-Definition cset_disjoint_fvars (c1 c2 :captureset) : Prop :=
-  match c1 , c2 with
-  | (cset_set A1 N1), (cset_set A2 N2) => AtomSet.F.Empty (AtomSet.F.inter A1 A2)
-  | _ , _ => True
-  end.
+Definition cset_references_univ_dec := cset_has_universal.
+Definition cset_references_univ (c : cap) :=
+    cset_references_univ_dec c = true.
 
 (** Capture set unions are what you'd expect. *)
-Definition cset_union (c1 c2 : captureset) : captureset :=
-  match c1 , c2 with
-  | _ , cset_universal => cset_universal
-  | cset_universal , _ => cset_universal
-  | cset_set A1 N1 , cset_set A2 N2 => cset_set (AtomSet.F.union A1 A2) (NatSet.F.union N1 N2)
+Definition cset_union (c1 c2 : cap) : cap :=
+  cset_set 
+    (AtomSet.F.union (cset_fvars c1) (cset_fvars c2))
+    (NatSet.F.union (cset_bvars c1) (cset_bvars c2))
+    ((cset_has_universal c1) || (cset_has_universal c2)).
+
+Definition cset_subset_dec (C D : cap) :=
+  AtomSet.F.subset (cset_fvars C) (cset_fvars D) 
+    && NatSet.F.subset (cset_bvars C) (cset_bvars D)
+    && (implb (cset_has_universal C) (cset_has_universal D)).
+
+(** ************************************************** *)
+(** Logical Predicates *)
+(** ************************************************** *)
+
+Definition cset_empty (c : cap) : Prop :=
+  AtomSet.F.Empty (cset_fvars c) /\ NatSet.F.Empty (cset_bvars c) /\ 
+    ((cset_has_universal c) = false). 
+
+Definition cset_subset_prop (c : cap) (d : cap) : Prop :=
+  AtomSet.F.Subset (cset_fvars c) (cset_fvars d) 
+    /\ NatSet.F.Subset (cset_bvars c) (cset_bvars d) 
+    /\  (leb (cset_has_universal c) (cset_has_universal d)).
+
+
+(** ************************************************** *)
+(** Properties *)
+(** ************************************************** *)
+
+Section Props.
+
+  Variable x y a f : atom.
+  Variable l m R : bool.
+  Variable A A1 A2 : atoms.
+  Variable k n : nat.
+  Variable N N1 N2 : nats.
+  Variable C D C1 C2 C3 : cap.
+
+  Lemma cset_bvar_mem_iff : 
+    cset_references_bvar k C <-> cset_references_bvar_dec k C = true.
+  Proof.  
+    destruct C ;
+      unfold cset_references_bvar, cset_references_bvar_dec in *; 
+      simpl in *; intuition.
+  Qed.
+
+  Lemma cset_fvar_mem_iff :
+    cset_references_fvar a C <-> cset_references_fvar_dec a C = true.
+  Proof.  
+    destruct C ;
+      unfold cset_references_fvar, cset_references_fvar_dec in *; 
+      simpl in *; intuition.
+  Qed.
+
+  Lemma cset_univ_mem_iff :
+    cset_references_univ C <-> cset_references_univ_dec C = true.
+  Proof.  
+    destruct C; unfold cset_references_univ, cset_references_univ_dec in *.
+    reflexivity.
+  Qed.
+
+  Lemma cset_bvar_not_mem_iff : 
+    ~ cset_references_bvar k C <-> cset_references_bvar_dec k C = false.
+  Proof.  
+    destruct C ;
+      unfold cset_references_bvar, cset_references_bvar_dec in *; split; intros; simpl in *; intuition.
+      rewrite <- NatSetFacts.not_mem_iff; fnsetdec.
+      rewrite <- NatSetFacts.not_mem_iff in H; fnsetdec.
+  Qed.
+
+  Lemma cset_fvar_not_mem_iff :
+    ~ cset_references_fvar a C <-> cset_references_fvar_dec a C = false.
+  Proof.  
+    destruct C ;
+      unfold cset_references_fvar, cset_references_fvar_dec in *; split; intros; simpl in *; intuition.
+      rewrite <- AtomSetFacts.not_mem_iff; fsetdec.
+      rewrite <- AtomSetFacts.not_mem_iff in H; fsetdec.
+  Qed.
+
+  Lemma cset_univ_not_mem_iff :
+    ~ cset_references_univ C <-> cset_references_univ_dec C = false.
+  Proof.  
+    destruct C; unfold cset_references_univ, cset_references_univ_dec, cset_has_universal in *; 
+      split.
+    intro; destruct b; auto*.
+    intro; subst; auto.
+  Qed.
+
+  Lemma fvars_1 : cset_fvars (cset_set A N R) = A.
+  Proof. unfold cset_fvars. trivial. Qed.
+
+  Lemma bvars_1 : cset_bvars (cset_set A N R) = N.
+  Proof. unfold cset_bvars. trivial. Qed.
+
+  Lemma lvars_1 : cset_has_universal (cset_set A N R) = R.
+  Proof. unfold cset_has_universal. trivial. Qed.
+
+  Lemma fvars_union_1 : cset_fvars (cset_union C D) = AtomSet.F.union (cset_fvars C) (cset_fvars D).
+  Proof. unfold cset_fvars. trivial. Qed.
+
+  Lemma bvars_union_1 : cset_bvars (cset_union C D) = NatSet.F.union (cset_bvars C) (cset_bvars D).
+  Proof. unfold cset_bvars. trivial. Qed.
+
+  Lemma lvars_union_1 : cset_has_universal (cset_union C D) = orb (cset_has_universal C) (cset_has_universal D).
+  Proof. unfold cset_has_universal. trivial. Qed.
+
+  Lemma remove_fvar_1 : cset_remove_fvar x (cset_set A N R) = (cset_set (AtomSet.F.remove x A) N R).
+  Proof. intros. unfold cset_remove_fvar in *; simpl in *. trivial. Qed.
+
+  Lemma remove_bvar_1 : cset_remove_bvar k (cset_set A N R) = (cset_set A (NatSet.F.remove k N) R).
+  Proof. intros. unfold cset_remove_bvar in *; simpl in *. trivial. Qed.
+
+  Lemma mem_bvar_1 : cset_references_bvar k C -> cset_references_bvar_dec k C = true.
+  Proof. rewrite cset_bvar_mem_iff; trivial. Qed.
+
+  Lemma mem_bvar_2 : cset_references_bvar_dec k C = true -> cset_references_bvar k C.
+  Proof. rewrite <- cset_bvar_mem_iff; trivial. Qed.
+
+  Lemma mem_fvar_1 : cset_references_fvar a C -> cset_references_fvar_dec a C = true.
+  Proof. rewrite cset_fvar_mem_iff; trivial. Qed.
+
+  Lemma mem_fvar_2 : cset_references_fvar_dec a C = true -> cset_references_fvar a C.
+  Proof. rewrite <- cset_fvar_mem_iff; trivial. Qed.
+
+  Lemma mem_lvar_1 : cset_references_univ C -> cset_references_univ_dec C = true.
+  Proof. rewrite cset_univ_mem_iff; trivial. Qed.
+
+  Lemma mem_lvar_2 : cset_references_univ_dec C = true -> cset_references_univ C.
+  Proof. rewrite <- cset_univ_mem_iff; trivial. Qed.
+
+  Lemma In_bvar_1 : k = n -> cset_references_bvar k C -> cset_references_bvar n C.
+  Proof. intros; subst; trivial. Qed.
+
+  Lemma In_fvar_1 : a = f -> cset_references_fvar a C -> cset_references_fvar f C.
+  Proof. intros; subst; trivial. Qed.
+
+  Lemma Is_empty : cset_empty empty_cset.
+  Proof. repeat split. fsetdec. fnsetdec. Qed.
+
+  Lemma union_fvar_1 : cset_references_fvar x (cset_union C D) -> cset_references_fvar x C \/ cset_references_fvar x D.
+  Proof. intros. unfold cset_union, cset_references_fvar in *; simpl in *. fsetdec. Qed.
+
+  Lemma union_fvar_2 : cset_references_fvar x C -> cset_references_fvar x (cset_union C D).
+  Proof. unfold cset_union, cset_references_fvar in *; simpl in *. fsetdec. Qed.
+
+  Lemma union_fvar_3 : cset_references_fvar x D -> cset_references_fvar x (cset_union C D).
+  Proof. unfold cset_union, cset_references_fvar in *; simpl in *. fsetdec. Qed.
+
+  Lemma union_bvar_1 : cset_references_bvar k (cset_union C D) -> cset_references_bvar k C \/ cset_references_bvar k D.
+  Proof. intros. unfold cset_union, cset_references_bvar in *; simpl in *. fnsetdec. Qed.
+
+  Lemma union_bvar_2 : cset_references_bvar k C -> cset_references_bvar k (cset_union C D).
+  Proof. unfold cset_union, cset_references_bvar in *; simpl in *. fnsetdec. Qed.
+
+  Lemma union_bvar_3 : cset_references_bvar k D -> cset_references_bvar k (cset_union C D).
+  Proof. unfold cset_union, cset_references_bvar in *; simpl in *. fnsetdec. Qed.
+
+  Lemma union_lvar_1 : cset_references_univ (cset_union C D) -> 
+    cset_references_univ C \/ cset_references_univ D.
+  Proof. intros. unfold cset_union, cset_references_univ in *; simpl in *.
+    rewrite orb_true_iff in H; auto*.
+  Qed.
+
+  Lemma union_lvar_2 : cset_references_univ C -> cset_references_univ (cset_union C D).
+  Proof. unfold cset_union, cset_references_univ in *; simpl in *. intro.
+    rewrite orb_true_iff. auto. Qed.
+
+  Lemma union_lvar_3 : cset_references_univ D -> cset_references_univ (cset_union C D).
+  Proof. unfold cset_union, cset_references_univ in *; simpl in *. intro.
+    rewrite orb_true_iff. auto. Qed.
+
+  Lemma union_sub_1 : cset_subset_prop C D -> cset_union D C = D.
+  Proof. 
+    unfold cset_union, cset_subset_prop, cset_fvars, cset_bvars, cset_has_universal. 
+    intros. destruct C; destruct D; simpl; f_equal.
+    fsetdec. fnsetdec.
+      destruct b; destruct b0; auto*.
+  Qed.
+  
+  Lemma union_sub_2 : cset_subset_prop C D -> D = cset_union D C.
+  Proof. 
+    unfold cset_union, cset_subset_prop, cset_fvars, cset_bvars, cset_has_universal. 
+    intros. destruct C; destruct D; simpl; f_equal.
+    fsetdec. fnsetdec.
+      destruct b; destruct b0; auto*.
+  Qed.
+
+  Lemma union_subset_distribute_1 : cset_subset_prop C1 C2 -> cset_subset_prop (cset_union C1 D) (cset_union C2 D).
+  Proof. 
+    intros. unfold cset_subset_prop in *; inversion H as [Sub_F [Sub_B Sub_A]];
+    unfold cset_union, cset_fvars, cset_bvars, cset_has_universal, cset_fvar in *; destruct C1; destruct C2.
+    repeat split; try fsetdec; try fnsetdec.
+      destruct b; destruct b0; unfold leb in *; simpl in *; destruct D; destruct b; auto*.
+  Qed.
+
+End Props.
+
+(* TODO defined here to avoid all the implicit arguments *)
+Lemma subset_univ_1 : forall R C, 
+  cset_subset_prop R C -> cset_references_univ R -> cset_references_univ C.
+Proof. unfold cset_references_univ, cset_subset_prop; intros.
+  destruct H as [_ [_ H]]. unfold cset_has_universal, cset_references_univ_dec in *; destruct R;
+    destruct C; unfold cset_has_universal, leb in *; destruct b; destruct b0; auto*. Qed.
+
+Hint Rewrite 
+  fvars_1 bvars_1 lvars_1 
+  fvars_union_1 bvars_union_1 lvars_union_1 
+  remove_fvar_1 remove_bvar_1 
+: csets.
+
+
+Hint Resolve 
+  mem_bvar_1 mem_fvar_1 Is_empty 
+  union_fvar_1 union_fvar_2 union_fvar_3 
+  union_bvar_1 union_bvar_2 union_bvar_3
+  union_lvar_1 union_lvar_2 union_lvar_3 
+  union_sub_1 union_sub_2 union_subset_distribute_1
+  subset_univ_1
+: core.
+
+Hint Immediate In_bvar_1 In_fvar_1 mem_bvar_2 mem_fvar_2 mem_lvar_2 : core.
+
+(* Some subset properties *)
+Lemma subset_refl : forall C,
+  cset_subset_prop C C.
+Proof.
+  intros. unfold cset_subset_prop. repeat split. fsetdec. fnsetdec.
+    unfold leb; destruct C; unfold cset_has_universal; destruct b; auto*.
+Qed.
+
+Lemma subset_union_left : forall C1 C2,
+  cset_subset_prop C1 (cset_union C1 C2).
+Proof.
+  intros. destruct C1. destruct C2. unfold cset_subset_prop, cset_union, cset_fvars,
+    cset_bvars, cset_has_universal. repeat split. fsetdec. fnsetdec.
+    unfold leb; destruct b; destruct b0; auto*.
+Qed.
+
+Lemma subset_union_right : forall C1 C2,
+  cset_subset_prop C2 (cset_union C1 C2).
+Proof.
+  intros. destruct C1. destruct C2. unfold cset_subset_prop, cset_union, cset_fvars,
+    cset_bvars, cset_has_universal. repeat split. fsetdec. fnsetdec.
+    unfold leb; destruct b; destruct b0; auto*. 
+Qed.
+
+Lemma subset_trans : forall A B C,
+  cset_subset_prop A B -> cset_subset_prop B C -> cset_subset_prop A C.
+Proof.
+  intros * AB BC.
+  inversion AB as [ABF [ABN ABL]]; subst; inversion BC as [BCF [BCN BCL]]; subst...
+  repeat (econstructor; try fsetdec; try fnsetdec)...
+Qed.
+
+Hint Immediate subset_union_left subset_union_right  subset_refl: core.
+
+
+(***********)
+(* Tactics *)
+(***********)
+
+Ltac rewrite_set_facts_in H :=
+  match type of H with
+  | true = _ => symmetry in H
+  | false = _ => symmetry in H
+  | _ => idtac
+  end;
+  match type of H with
+  | NatSet.F.mem _ _ = true => rewrite <- NatSetFacts.mem_iff in H
+  | NatSet.F.mem _ _ = false => rewrite <- NatSetFacts.not_mem_iff in H
+  | AtomSet.F.mem _ _ = true => rewrite <- AtomSetFacts.mem_iff in H
+  | AtomSet.F.mem _ _ = false => rewrite <- AtomSetFacts.not_mem_iff in H
+  | LabelSet.F.mem _ _ = true => rewrite <- LabelSetFacts.mem_iff in H
+  | LabelSet.F.mem _ _ = false => rewrite <- LabelSetFacts.not_mem_iff in H
+  | cset_references_bvar_dec _ _ = true => rewrite <- cset_bvar_mem_iff in H
+  | cset_references_fvar_dec _ _ = true => rewrite <- cset_fvar_mem_iff in H
+  | cset_references_lvar_dec _ _ = true => rewrite <- cset_lvar_mem_iff in H
+  | cset_references_bvar_dec _ _ = false => rewrite <- cset_bvar_not_mem_iff in H
+  | cset_references_fvar_dec _ _ = false => rewrite <- cset_fvar_not_mem_iff in H
+  | cset_references_lvar_dec _ _ = false => rewrite <- cset_lvar_not_mem_iff in H
   end.
 
-(** Empty capture sets / universal capture sets *)
-Definition cset_empty (c : captureset) : Prop :=
-  match c with
-  | cset_universal => False
-  | cset_set A N => empty_cset_bvars c /\ empty_cset_fvars c
+Ltac rewrite_set_facts_back_in H :=
+  match type of H with
+  | true = _ => symmetry in H
+  | false = _ => symmetry in H
+  | _ => idtac
+  end;
+  match type of H with
+  | NatSet.F.In _ _          => rewrite -> NatSetFacts.mem_iff in H
+  | (~ NatSet.F.In _ _)      => rewrite -> NatSetFacts.not_mem_iff in H
+  | AtomSet.F.In _ _         => rewrite -> AtomSetFacts.mem_iff in H
+  | (~ AtomSet.F.In _ _)     => rewrite -> AtomSetFacts.not_mem_iff in H
+  | LabelSet.F.In _ _         => rewrite -> LabelSetFacts.mem_iff in H
+  | (~ LabelSet.F.In _ _)     => rewrite -> LabelSetFacts.not_mem_iff in H
+  | cset_references_bvar _ _ => rewrite -> cset_bvar_mem_iff in H
+  | cset_references_fvar _ _ => rewrite -> cset_fvar_mem_iff in H
+  | cset_references_lvar _ _ => rewrite -> cset_lvar_mem_iff in H
+  | (~ cset_references_bvar _ _) => rewrite -> cset_bvar_not_mem_iff in H
+  | (~ cset_references_fvar _ _) => rewrite -> cset_fvar_not_mem_iff in H
+  | (~ cset_references_lvar _ _) => rewrite -> cset_lvar_not_mem_iff in H
   end.
 
-Definition cset_remove_bvar (k : nat) (c : captureset) : captureset :=
-  match c with
-  | cset_universal => cset_universal
-  | cset_set AC NC => cset_set AC (NatSet.F.remove k NC)
+
+Ltac simpl_in_cset :=
+  let go H := rewrite_set_facts_back_in H; try rewrite H in *; rewrite_set_facts_in H in
+  match goal with
+  | H: cset_references_bvar_dec ?I ?C = ?B |- _ => try rewrite H in *
+  | H: ~ (cset_references_bvar _ _) |- _ => go H
+  | H: (cset_references_bvar _ _)   |- _ => go H
+  | H: ~ (cset_references_fvar _ _) |- _ => go H
+  | H: (cset_references_fvar _ _)   |- _ => go H
+  | H: ~ (cset_references_lvar _ _) |- _ => go H
+  | H: (cset_references_lvar _ _)   |- _ => go H
   end.
 
-Definition cset_remove_fvar (a : atom) (c : captureset) : captureset :=
-  match c with
-  | cset_universal => cset_universal
-  | cset_set AC NC => cset_set (AtomSet.F.remove a AC) NC
+Ltac destruct_set_mem a bs :=
+  match type of bs with
+  | AtomSet.F.t =>
+    let H := fresh a "In" in
+    destruct (AtomSet.F.mem a bs) eqn:H; rewrite_set_facts_in H
+  | NatSet.F.t =>
+    let H := fresh a "In" in
+    destruct (NatSet.F.mem a bs) eqn:H; rewrite_set_facts_in H
+  | LabelSet.F.t =>
+    let H := fresh a "In" in
+    destruct (LabelSet.F.mem a bs) eqn:H; rewrite_set_facts_in H
+  | cap =>
+    match type of a with
+    | atom => 
+      let H := fresh a "In" in
+      destruct (cset_references_fvar_dec a bs) eqn:H; rewrite_set_facts_in H; trivial
+    | nat =>
+      let H := fresh a "In" in
+      destruct (cset_references_bvar_dec a bs) eqn:H; rewrite_set_facts_in H; trivial
+    | label => 
+      let H := fresh a "In" in
+      destruct (cset_references_lvar_dec a bs) eqn:H; rewrite_set_facts_in H; trivial
+    end
   end.
+
+
+Lemma funion_empty_idempotent : forall xs,
+    NatSet.F.union xs {}N = xs.
+Proof. intros. fnsetdec. Qed.
+
+Lemma empty_funion_idempotent : forall xs,
+    NatSet.F.union {}N xs = xs.
+Proof. intros. fnsetdec. Qed.
+
+Lemma union_empty_idempotent : forall xs,
+    AtomSet.F.union xs {} = xs.
+Proof. intros. fsetdec. Qed.
+
+Lemma empty_union_idempotent : forall xs,
+    AtomSet.F.union {} xs = xs.
+Proof. intros. fsetdec. Qed.
+
+Lemma lunion_empty_idempotent : forall xs,
+    LabelSet.F.union xs {}L = xs.
+Proof. intros. lsetdec. Qed.
+
+Lemma empty_lunion_idempotent : forall xs,
+    LabelSet.F.union {}L xs = xs.
+Proof. intros. lsetdec. Qed.
+
+Hint Rewrite 
+  funion_empty_idempotent empty_funion_idempotent 
+  union_empty_idempotent empty_union_idempotent 
+  lunion_empty_idempotent empty_lunion_idempotent 
+: csets.
+
+Lemma cunion_empty_idempotent : forall xs,
+    cset_union xs {}C = xs.
+Proof. intros. destruct xs. unfold cset_union. autorewrite with csets; trivial. Qed.
+
+Lemma empty_cunion_idempotent : forall xs,
+    cset_union {}C xs = xs.
+Proof. intros. destruct xs. unfold cset_union. autorewrite with csets; trivial. Qed.
+
+Hint Rewrite cunion_empty_idempotent empty_cunion_idempotent : csets.
+
+Ltac csetsimpl :=
+  try (progress (simpl; autorewrite with csets in *); intuition csetsimpl).
+
+Ltac csetsimplIn H :=
+  try (progress (simpl in H; autorewrite with csets in H); intuition (csetsimplIn H)).
+
+Tactic Notation "csetsimpl" "in" hyp(H) := csetsimplIn H.
+
+Ltac csetdec := csetsimpl; try fsetdec; try fnsetdec.
+
+
+
+(** ************************************************** *)
+(** Locally Namelesss *)
+(** ************************************************** *)
+
+
+Definition capt (c : cap) : Prop := NatSet.F.Empty (cset_bvars c).
+
+Lemma singleton_closed : forall f,
+  capt (cset_fvar f).
+Proof.
+  unfold capt, cset_fvar; fnsetdec. 
+Qed.
+
+Lemma capt_empty_bvar : forall A N R,
+  capt (cset_set A N R) ->
+  N = {}N.
+Proof.
+  intros. unfold capt, cset_fvar in *. fnsetdec. 
+Qed.
+
+Hint Unfold capt : core.
+Hint Resolve capt_empty_bvar : core.
 
 
 (** Opening a capture set with a bound variable d[k -> c] *)
-Definition open_cset (k : nat) (c : captureset) (d : captureset) : captureset :=
-  if cset_references_bvar_dec k d then
+Definition open_cset (k : nat) (c : cap) (d : cap) : cap :=
+  if cset_references_bvar_dec k d then 
     cset_union c (cset_remove_bvar k d)
-  else
+  else 
     d.
 
 (** Substituting a capture set with a free variable d[a -> c] *)
-Definition subst_cset (a : atom) (c : captureset) (d: captureset) : captureset :=
+Definition subst_cset (a : atom) (c : cap) (d: cap) : cap :=
   if cset_references_fvar_dec a d then
     cset_union c (cset_remove_fvar a d)
   else
     d.
 
-(* TODO rename to cset_subset *)
-(** Predicates around subsets, and decidability for destruction *)
-Inductive cset_subset_prop : captureset -> captureset -> Prop :=
-| cset_subset_univ : forall c, cset_subset_prop c cset_universal
-| cset_subset_elem : forall ac nc ad nd,
-  AtomSet.F.Subset ac ad -> NatSet.F.Subset nc nd -> cset_subset_prop (cset_set ac nc) (cset_set ad nd)
-.
-
-Definition cset_subset_dec (c d : captureset) :=
-  match c , d with
-  | _ , cset_universal => true
-  | cset_universal , _ => false
-  | cset_set AC NC , cset_set AD ND => AtomSet.F.subset AC AD && NatSet.F.subset NC ND
-  end.
-
-(** A helper, to eliminate terms like <complex computation> && false *)
-Local Lemma reduce_false (b : bool) : b && false = false.
+Lemma subst_over_subset : forall C1 C2 D x,
+  cset_subset_prop C1 C2 -> 
+  cset_subset_prop (subst_cset x D C1) (subst_cset x D C2).
 Proof.
-destr_bool.
+  intros.
+  unfold cset_subset_prop in *.
+  destruct H as [HF [HB HL]].
+  unfold subst_cset, cset_references_fvar_dec; destruct C1; destruct C2; simpl in *.
+    destruct_set_mem x t; destruct_set_mem x t2; simpl in *; repeat split;
+    try fsetdec; try fnsetdec; try lsetdec; exfalso; fsetdec.
 Qed.
 
-(** Why isn't this part of the standard library? **)
-Local Lemma eliminate_false (b : bool) : (b = false) <-> (b <> true).
+Lemma subst_subset_intro : forall C1 C2 x,
+  (* C1 is closed *)
+  capt C1 ->
+  cset_subset_prop (cset_fvar x) C2 ->
+  cset_subset_prop C1 (subst_cset x C1 C2).
 Proof.
-destr_bool; split; destr_bool.
-contradict H; trivial.
+  intros.
+  destruct C2.
+  (* TODO what can we do to prevent having to unfold? *)
+  unfold capt in H.
+  unfold cset_subset_prop, subst_cset, cset_references_fvar_dec in *.
+  destruct H0 as [HF [HB HL]]; simpl in *; csetsimpl; destruct_set_mem x t; csetsimpl;
+    try fsetdec;
+    try fnsetdec;
+    try lsetdec.
+  unfold AtomSet.F.Subset in HF. specialize (HF x). fsetdec.
 Qed.
 
-(** Two relations relating the subset relation to the subset computation. *)
-Lemma cset_subset_iff (c1 c2 : captureset) : cset_subset_prop c1 c2 <-> cset_subset_dec c1 c2 = true.
-Proof.
-  split.
-  (* --> *)
-  * intro. inversion H ; unfold cset_subset_dec.
-    - subst. destruct c1 ; eauto.
-    - subst.
-      rewrite NatSetFacts.subset_iff in *. rewrite AtomSetFacts.subset_iff in *.
-      rewrite H0. rewrite H1. auto.
-  (* <-- *)
-  * intro. unfold cset_subset_dec in H.
-    destruct c1 eqn:H1 ; destruct c2 eqn:H2.
-    - apply cset_subset_univ.
-    - discriminate H.
-    - apply cset_subset_univ.
-    - apply cset_subset_elem ; rewrite andb_true_iff in H ; destruct H ;
-      rewrite <- NatSetFacts.subset_iff in * ; rewrite <- AtomSetFacts.subset_iff in * ; auto.
+Lemma subst_cset_union : forall x D C1 C2,
+  subst_cset x D (cset_union C1 C2) = (cset_union (subst_cset x D C1) (subst_cset x D C2)).
+Proof with eauto.
+  intros.
+  unfold subst_cset, cset_fvars, cset_union, cset_fvar, cset_references_fvar_dec, cset_remove_fvar; simpl in *.
+  destruct C1; destruct C2; destruct D; simpl.
+  destruct_set_mem x (t `union` t2); destruct_set_mem x t; destruct_set_mem x t2;
+    unfold cset_bvars, cset_fvars, cset_lvars; f_equal; try fsetdec; try fnsetdec; try lsetdec...
 Qed.
 
-Lemma cset_subset_not_iff (c1 c2 : captureset) : ~ cset_subset_prop c1 c2 <-> cset_subset_dec c1 c2 = false.
+Lemma subst_cset_singleton : forall x C,
+  subst_cset x C (cset_fvar x) = C.
+Proof.
+  unfold subst_cset, cset_fvar, cset_fvars, cset_references_fvar_dec, cset_remove_fvar in *; simpl.
+  intros.
+  destruct_set_mem x (singleton x).
+  replace (singleton x `remove` x) with {}; try fsetdec.
+  destruct C; unfold cset_union; simpl; autorewrite with csets; trivial.
+  fsetdec.
+Qed.
+
+Lemma subst_cset_fresh : forall x C1 C2,
+  x `notin` (cset_fvars C1) ->
+  C1 = subst_cset x C2 C1.
+Proof with eauto.
+  intros.
+  unfold subst_cset, cset_references_fvar_dec, cset_union, cset_remove_fvar, cset_fvars in *.
+  destruct C1 eqn:HC; destruct C2 eqn:HC2;
+  destruct_set_mem x t...
+  notin_solve.
+Qed.
+
+Lemma singleton_lvar : forall l,
+  cset_references_lvar l (cset_lvar l).
+Proof.
+  unfold cset_references_lvar, cset_lvars, cset_lvar; lsetdec.
+Qed.
+
+Lemma subst_cset_fresh_id : forall x X C,
+  x <> X ->
+  (subst_cset X C (cset_fvar x)) = (cset_fvar x).
+Proof.
+  intros. unfold cset_fvar, subst_cset, cset_references_fvar_dec, cset_fvars.
+  destruct_set_mem X (singleton x); auto.
+  assert (x = X) by fsetdec; fsetdec.
+Qed.
+
+Lemma subst_cset_union_id : forall x y D C1,
+  x <> y ->
+  subst_cset x D (cset_union C1 (cset_fvar y)) = (cset_union (subst_cset x D C1) (cset_fvar y)).
+Proof with eauto.
+  intros.
+  rewrite <- (subst_cset_fresh_id y x D) at 2...
+  apply subst_cset_union.
+Qed.
+
+Lemma subst_cset_lvar : forall x C l R,
+  cset_references_lvar l R ->
+  cset_references_lvar l (subst_cset x C R).
+Proof with eauto.
+  destruct R; unfold cset_lvars, subst_cset, cset_references_lvar, cset_lvars, cset_references_fvar_dec, cset_remove_fvar, cset_union in *; simpl.
+  destruct_set_mem x t; try lsetdec.
+Qed.
+
+Lemma subst_cset_lvar_idempotent : forall x C l,
+  (subst_cset x C (cset_lvar l)) = (cset_lvar l).
+Proof with eauto.
+  unfold cset_lvar, subst_cset, cset_references_fvar_dec, cset_union, cset_fvars, cset_lvars, cset_bvars. csetsimpl.
+  destruct C; destruct_set_mem x {}... fsetdec.
+Qed.
+
+Lemma open_cset_capt : forall i C c,
+  capt C ->
+  C = open_cset i c C.
+Proof with eauto*.
+  intros i C c H.  
+  unfold open_cset in *.
+  destruct_set_mem i C. 
+  exfalso. unfold capt, cset_references_bvar in *. 
+  assert (~ NatSet.F.In i (cset_bvars C)) by nnotin_solve...
+Qed.
+
+Lemma subst_cc_intro_rec : forall X (C : cap) U k,
+  X `notin` (cset_fvars C) ->
+  open_cset k U C = subst_cset X U (open_cset k (cset_fvar X) C).
 Proof with auto*.
-  split.
-  * intro H. rewrite eliminate_false. contradict H. apply cset_subset_iff...
-  * intro H. rewrite eliminate_false in H. contradict H. apply cset_subset_iff...
-Qed.
+  intros * NotIn.
+  destruct C. destruct U. 
+  unfold open_cset, cset_references_bvar_dec, 
+    subst_cset, cset_bvars, cset_remove_bvar, cset_remove_fvar, cset_references_fvar_dec, cset_fvars in *; simpl.
 
-(* TODO move to CaptureSets. *)
-Lemma cset_subset_reflexivity (c : captureset) : cset_subset_prop c c.
-Proof with auto.
-  rewrite cset_subset_iff.
-  unfold cset_subset_dec.
-  destruct c...
-  assert (AtomSet.F.subset t t = true). { rewrite <- AtomSetFacts.subset_iff. fsetdec. }
-  assert (NatSet.F.subset t0 t0 = true). { rewrite <- NatSetFacts.subset_iff. fnsetdec. }
-  intuition.
-Qed.
-
-(* unversals can't be subcaptres of concrete capture sets. *)
-Lemma cset_universal_subset : forall tf tb,
-  cset_subset_prop cset_universal (cset_set tf tb) ->
-  False.
-Proof with auto.
-  intros tf tb H.
-  inversion H...
+  destruct_set_mem k t0; simpl. autorewrite with csets.
+  unfold cset_union, cset_fvars.
+  destruct_set_mem X (singleton X `union` t); simpl; autorewrite with csets; f_equal;
+    try fsetdec; try lsetdec.
+  
+  destruct_set_mem X t; auto.
+  fsetdec.
 Qed.
 
 
-(* Some simple tactics to work with capture sets *)
+Hint Resolve singleton_closed singleton_lvar open_cset_capt subst_cset_lvar : core.
+Hint Rewrite subst_cset_singleton subst_cset_union subst_cset_lvar_idempotent : csets.
 
-(* Uses hypothesis about capture set inclusion to rewrite hyps and goal *)
-Ltac simpl_in_cset :=
-  match goal with
-    H: cset_references_bvar_dec ?I ?C = ?B
-    |- _ => rewrite H in *
-  end.
 
-(* Rewrites hypothesis by unfolding cset definitions and using hypothesis about
-   inclusion. *)
-Ltac csethyp := try autounfold with cset_scope in *; try simpl_in_cset.
+(* unfold subst_cb, subst_cset, cset_references_fvar_dec, cset_fvar, cset_remove_fvar, cset_union.  
+  destruct C1; destruct_set_mem X (singleton x)... fsetdec. *)
+  
+Lemma open_cset_rec_capt_aux : forall c j V i U,
+  i <> j ->
+  capt V ->
+  (* TODO probably, we also want disjointness of labels here? *)
+  (cset_fvars V) `disjoint` (cset_fvars U) ->
+  labels_disjoint (cset_lvars V) (cset_lvars U) ->
+  open_cset j V c = open_cset i U (open_cset j V c) ->
+  c = open_cset i U c.
+Proof with eauto.
+  intros * Hfresh Hempty HdisjointV HdisjointL.
+  unfold cset_fvars, disjoint, labels_disjoint, capt, open_cset, cset_remove_bvar, cset_references_bvar_dec, cset_union,
+    cset_bvars, cset_lvars in *.
+  destruct c eqn:Hc; destruct U eqn:HU; destruct V eqn:HV; destruct_set_mem j t0; unfold cset_fvars in *;
+    destruct_set_mem i t0;
+    destruct (NatSet.F.mem i (NatSet.F.union t6 (NatSet.F.remove j t0))) eqn:iInUnion;
+    rewrite_set_facts_in iInUnion;
+    intro Heq;
+    inversion Heq; f_equal; assert (t6 = {}N) by fnsetdec; subst; autorewrite with csets in *; try fsetdec; try fnsetdec; try lsetdec...
+  * assert (t2 `subset` t). {
+      intros e Het1.
+      assert (e `in` (t2 `union` t5 `union` t)) by fsetdec.
+      assert (e `notin` t5) by fsetdec.
+      rewrite <- H0 in H. fsetdec.
+    }
+    fsetdec.
+  * assert (NatSet.F.In i (NatSet.F.remove j t0)) by fnsetdec.
+    assert (~NatSet.F.In i (NatSet.F.remove i (NatSet.F.remove j t0))) by fnsetdec.
+    assert (NatSet.F.In i t3). {
+      destruct_set_mem i t3...
+      exfalso.
+      assert (~ NatSet.F.In i (NatSet.F.union t3 (NatSet.F.remove i (NatSet.F.remove j t0)))) by fnsetdec.
+      rewrite <- H1 in H4. fnsetdec.
+    }
+    assert (NatSet.F.Subset t3 t0). {
+      intros e Het3.
+      destruct (e === i); subst...
+      assert (NatSet.F.In e (NatSet.F.union t3 (NatSet.F.remove i (NatSet.F.remove j t0)))) by fnsetdec.
+      rewrite <- H1 in H5...
+      assert (e <> j) by fnsetdec.
+      fnsetdec.
+    }
+    fnsetdec.
+  * assert (LabelSet.F.Subset t4 t1). {
+      intros e Het4.
+      assert (LabelSet.F.In e (LabelSet.F.union t4 (LabelSet.F.union t7 t1))) by lsetdec.
+      assert (~ LabelSet.F.In e t7) by lsetdec.
+      rewrite <- H2 in H. lsetdec.
+    }
+    lsetdec.
+Qed.
 
-(* Uses facts about the underlying sets to simplify hypothesis and solve the goal *)
-Ltac csetdec := repeat (
-  try csethyp ;
-  (try rewrite <- NatSetFacts.mem_iff in * ; try fnsetdec) ||
-  (try rewrite <- AtomSetFacts.mem_iff in * ; try fsetdec)
-).
+Lemma subst_cset_open_cset_rec : forall x k C1 C2 D,
+  capt C1 ->
+  subst_cset x C1 (open_cset k C2 D) = open_cset k (subst_cset x C1 C2) (subst_cset x C1 D).
+Proof with eauto*.
+  intros x k C1 C2 D Closed.
+  destruct D eqn:Hc; destruct C1 eqn:HC1; destruct C2 eqn:HC2;
+  unfold capt, subst_cset, open_cset, cset_references_fvar_dec,
+    cset_references_bvar_dec, cset_remove_bvar, cset_remove_fvar, cset_union, cset_fvars, cset_bvars, cset_lvars in *; subst; csetsimpl.
 
-Hint Constructors cset_subset_prop : core.
+    assert (t3 = {}N) by fnsetdec; subst.
 
-Hint Transparent
-  cset_references_bvar cset_references_fvar
-  cset_remove_bvar cset_remove_fvar open_cset subst_cset
-  disjoint
-: cset_scope.
+    autorewrite with csets.
 
-Hint Unfold
-  cset_union cset_subset_dec
-  cset_remove_bvar cset_remove_fvar
-  open_cset subst_cset
-  cset_references_bvar cset_references_fvar
-  cset_all_fvars cset_all_bvars
-  disjoint
-: cset_scope.
+    destruct (NatSet.F.mem k t0) eqn:kT0;
+    destruct (AtomSet.F.mem x t) eqn:xT;
+    destruct (AtomSet.F.mem x t5) eqn:xT3;
+    destruct (AtomSet.F.mem x (t5 `union` t)) eqn:xUnion;
+    f_equal;
+    rewrite_set_facts_in kT0;
+    rewrite_set_facts_in xT;
+    rewrite_set_facts_in xT3;
+    rewrite_set_facts_in xUnion;
+    try fsetdec; try fnsetdec; try lsetdec;
+    rewrite_set_facts_back_in kT0; try rewrite kT0; rewrite_set_facts_in kT0; f_equal; try fsetdec; try fnsetdec; try lsetdec.
+Qed.
